test/ctypes/Client.ml
@@ -21,11 +21,11 @@ let replicate (n: Unsigned.UInt32.t): Lowlevel.tr = Lowlevel.replicate n
 let maybe_double (n: Lowlevel.int_opt ptr): unit = Lowlevel.maybe_double n
 
 
-(* let make_L (x: Unsigned.UInt32.t): Lowlevel.eith = Lowlevel.make_L x
- * 
- * let make_R (x: Unsigned.UInt16.t): Lowlevel.eith = Lowlevel.make_R x
- * 
- * let flip_t (p: Lowlevel.eith ptr): unit = Lowlevel.flip_t p *)
+let make_L (x: Unsigned.UInt32.t): Lowlevel.eith = Lowlevel.make_L x
+
+let make_R (x: Unsigned.UInt16.t): Lowlevel.eith = Lowlevel.make_R x
+
+let flip_t (p: Lowlevel.eith ptr): unit = Lowlevel.flip_t p
 
 
 let point_to_tuple (p: Lowlevel.point) =
@@ -81,4 +81,19 @@ let _ =
   maybe_double n_ptr;
   let v = !@ n_ptr in
   assert (getf v int_opt_tag = int_opt_tags_IntSome && getf v int_opt__0 = Unsigned.UInt32.of_int 24)
+
+let _ =
+  let open Lowlevel in
+  let arg1 = (Unsigned.UInt32.of_int 5) in
+  let e1 = make_L arg1 in
+  assert (getf e1 eith_tag = eith_tags_L && getf (getf e1 eith_u) eith__u_case_L = arg1);
+
+  let arg2 = (Unsigned.UInt16.of_int 7) in
+  let e2 = make_R arg2 in
+  assert (getf e2 eith_tag = eith_tags_R && getf (getf e2 eith_u) eith__u_case_R = arg2);
+
+  let n_ptr = allocate Lowlevel.eith e2 in
+  flip_t n_ptr;
+  let v = !@ n_ptr in
+  assert (getf v eith_tag = eith_tags_L && getf (getf v eith_u) eith__u_case_L = Unsigned.UInt32.of_int 7)
 
