test/ctypes/Lowlevel.fst
@@ -75,25 +75,22 @@ let maybe_double opt =
   in
   upd opt 0ul v
 
+// Inductives: general compilation scheme
+noeq type eith = | L of U32.t | R of U16.t
+val make_L: x: U32.t -> St eith
+let make_L x = L x
 
-// Not supported:
+val make_R: x: U16.t -> St eith
+let make_R x = R x
 
-// // Inductives: general compilation scheme
-// noeq type eith = | L of U32.t | R of U16.t
-// val make_L: x: U32.t -> St eith
-// let make_L x = L x
-
-// val make_R: x: U16.t -> St eith
-// let make_R x = R x
-
-// val flip_t: p: B.pointer eith -> Stack unit
-//   (requires fun h -> B.live h p)
-//   (ensures fun h0 _ h1 -> True)
-// let flip_t p =
-//   let open U32 in
-//   let open LowStar.Monotonic.Buffer in
-//   let v = match B.index p 0ul with
-//     | L n -> R (FStar.Int.Cast.uint32_to_uint16 n)
-//     | R n -> L (FStar.Int.Cast.uint16_to_uint32 n)
-//   in
-//   upd p 0ul v
+val flip_t: p: B.pointer eith -> Stack unit
+  (requires fun h -> B.live h p)
+  (ensures fun h0 _ h1 -> True)
+let flip_t p =
+  let open U32 in
+  let open LowStar.Monotonic.Buffer in
+  let v = match B.index p 0ul with
+    | L n -> R (FStar.Int.Cast.uint32_to_uint16 n)
+    | R n -> L (FStar.Int.Cast.uint16_to_uint32 n)
+  in
+  upd p 0ul v
